Add initialization to MailAPI.
Add a boolean flag to Mail state which captures whether the locks have been
initialized yet, along with a new operation called "Open" to set this flag.
When the flag is false, any operation other than Open triggers undefined
behavior.

Finishing program execution unsets the flag, while crashing sets it (because
recovery will have initialized the locks, at least in the current
implementation, however arguably we should consider changing this).

Note: the invariants for the refinement proof need to be updated to reflect
that when this flag is false, the locks/global are not set up properly.

src/Examples/MailServer/MailAPI.v
@@ -15,6 +15,7 @@ Module Mail.
   Implicit Types (uid:uint64).
 
   Inductive Op : Type -> Type :=
+  | Open : Op unit
   | Pickup_Start uid : Op (list (string * list byte))
   | Pickup_End uid (msgs: list (string * list byte)) : Op (slice.t Message.t)
   | Deliver_Start uid (msg: slice.t byte) : Op unit
@@ -52,10 +53,12 @@ Module Mail.
 
   Record State : Type :=
     { heap: Data.State;
-      messages: gmap.gmap uint64 (MailboxStatus * gmap.gmap string (list byte)); }.
+      messages: gmap.gmap uint64 (MailboxStatus * gmap.gmap string (list byte));
+      open : bool;
+    }.
 
   Global Instance etaState : Settable _ :=
-    settable! Build_State <heap; messages>.
+    settable! Build_State <heap; messages; open>.
 
   Import RelationNotations.
 
@@ -107,7 +110,13 @@ Module Mail.
          _ <- puts (set heap (set Data.allocs (updDyn (a:=Ptr.Heap T) p.(slice.ptr) (s', alloc))));
          readSome (fun _ => Data.getSliceModel p alloc).
 
-  Definition step T (op: Op T) : relation State State T :=
+  Definition step_closed T (op: Op T) : relation State State T :=
+    match op in Op T return relation State State T with
+    | Open => puts (set open (λ _, true))
+    | _ => error
+    end.
+
+  Definition step_open T (op: Op T) : relation State State T :=
     match op in Op T return relation State State T with
     | Pickup_Start uid =>
       let! (s, msgs) <- lookup messages uid;
@@ -142,10 +151,22 @@ Module Mail.
            s <- Filesys.FS.unwrap (mailbox_lock_release s);
            puts (set messages <[uid := (s, msgs)]>)
     | DataOp op => _zoom heap (Data.step op)
+    | Open => error
     end.
 
-  Definition crash_step : relation State State unit := pure tt.
-  Definition finish_step : relation State State unit := pure tt.
+  Definition step T (op: Op T) : relation State State T :=
+    i <- reads open;
+    match i with
+    | true => step_open op
+    | false => step_closed op
+    end.
+
+  (* Post crash, recovery will perform lock initialization for the mailserver *)
+  Definition crash_step : relation State State unit :=
+    puts (set open (λ _, true)).
+
+  Definition finish_step : relation State State unit :=
+    puts (set open (λ _, false)).
 
   Definition sem : Dynamics Op State :=
     {| Proc.step := step;
@@ -154,6 +175,7 @@ Module Mail.
 
   Definition initP (s:State) :=
     s.(heap) = ∅ /\
+    s.(open) = false /\
     (forall (uid: uint64),
         (uid < 100 -> s.(messages) !! uid = Some (MUnlocked, ∅)) /\
         (uid >= 100 -> s.(messages) !! uid = None)).
